\documentclass[10pt,class=article,crop=false]{standalone}
\usepackage{../exo7formules}


\begin{document}



%%%%%%%%%%%%%%%%%%%%%%%%%%%%%%%%%%%%%%%%%%%%%%%%%%%%%%%%%%%%%%%%
\section{Formulaire: trigonom√©trie circulaire et hyperbolique}

\mycenterline{\textbf{Propri\'et\'es trigonom\'etriques}: remplacer $\cos$ par $\ch$
			et $\sin$ par $\ii\cdot\sh$.}

\begin{multicols}{2}
	
	$$\cos^2 x + \sin^2 x = 1$$
	
	\begin{align*}
		\cos(a+b)&=\cos a\cdot\cos b - \sin a\cdot\sin b\\
		\sin(a+b)&=\sin a\cdot\cos b  +  \sin b\cdot\cos a \\
		\tan (a+b)&=\frac{\tan a + \tan b}{1-\tan a\cdot\tan b} \\
	\end{align*}
	
	
	$$\ch^2 x - \sh^2 x = 1$$
	
	\begin{align*}
		\ch(a+b)&=\ch a\cdot\ch b + \sh a\cdot\sh b\\
		\sh(a+b)&=\sh a\cdot\ch b  +  \sh b\cdot\ch a\\
		\tanh (a+b)&=\frac{\tanh a + \tanh b}{1+\tanh a\cdot\tanh b}\\
	\end{align*}
\end{multicols}



\begin{multicols}{2}
	\begin{align*}
		\cos(a-b)&=\cos a\cdot\cos b + \sin a\cdot\sin b\\
		\sin(a-b)&=\sin a\cdot\cos b  - \sin b\cdot\cos a \\
		\tan (a-b)&=\frac{\tan a - \tan b}{1+\tan a\cdot\tan b} \\
	\end{align*}
	
	\begin{align*}
		\ch(a-b)&=\ch a\cdot\ch b - \sh a\cdot\sh b\\
		\sh(a-b)&=\sh a\cdot\ch b  - \sh b\cdot\ch a\\
		\tanh (a-b)&=\frac{\tanh a - \tanh b}{1-\tanh a\cdot\tanh b}\\
	\end{align*}
	
\end{multicols}

%\vspace{0.5cm}
\begin{multicols}{2}
	\begin{align*}
		\cos 2a &= 2\,\cos^2a-1\\
		&= 1-2\,\sin^2a\\
		&=\cos^2a-\sin^2a\\[3mm]
		\sin 2a &= 2\,\sin a\cdot\cos a\\[3mm]
		\tan 2a &= \frac{2\,\tan a}{1-\tan^2 a}
	\end{align*}
	
	\begin{align*}
		\ch 2a &= 2\,\ch^2a-1\\
		&= 1+2\,\sh^2a\\
		&=\ch^2a+\sh^2a\\[3mm]
		\sh 2a &= 2\,\sh a\cdot\ch a\\[3mm]
		\tanh 2a &= \frac{2\,\tanh a}{1+\tanh^2 a}
	\end{align*}
\end{multicols}


\begin{multicols}{2}
	\small
	\begin{align*}
		\cos a\cdot\cos b &= \frac{1}{2}\,\big[ \cos(a+b)+\cos(a-b)\big]\\
		\sin a\cdot\sin b &= \frac{1}{2}\,\big[ \cos(a-b)-\cos(a+b)\big]\\
		\sin a\cdot\cos b &= \frac{1}{2}\,\big[ \sin(a+b)+\sin(a-b)\big]
	\end{align*}
	
	\begin{align*}
		\ch a\cdot\ch b &= \frac{1}{2}\,\big[ \ch(a+b)+\ch(a-b)\big]\\
		\sh a\cdot\sh b &= \frac{1}{2}\,\big[ \ch(a+b)-\ch(a-b)\big]\\
		\sh a\cdot\ch b &= \frac{1}{2}\,\big[ \sh(a+b)+\sh(a-b)\big]
	\end{align*}
\end{multicols}



\begin{multicols}{2}
	\begin{align*}
		\cos p+\cos q &= 2\,\cos \frac{p+q}{2}\cdot\cos\frac{p-q}{2}\\
		\cos p-\cos q &= -2\,\sin \frac{p+q}{2}\cdot\sin \frac{p-q}{2}\\
		\sin p+\sin q &= 2\,\sin \frac{p+q}{2}\cdot\cos\frac{p-q}{2}\\
		\sin p-\sin q &= 2\,\sin \frac{p-q}{2}\cdot\cos\frac{p+q}{2}
	\end{align*}\vspace{0.1cm}
	\begin{align*}
		\ch p+\ch q &= 2\,\ch \frac{p+q}{2}\cdot\ch\frac{p-q}{2}\\
		\ch p-\ch q &= 2\,\sh \frac{p+q}{2}\cdot\sh \frac{p-q}{2}\\
		\sh p+\sh q &= 2\,\sh \frac{p+q}{2}\cdot\ch\frac{p-q}{2}\\
		\sh p-\sh q &= 2\,\sh \frac{p-q}{2}\cdot\ch\frac{p+q}{2}
	\end{align*}
\end{multicols}

%**********************************
%\newpage

\begin{multicols}{2}
	Avec \quad $t=\tan \frac{x}{2}$ \quad on a \quad
	$$
	\begin{cases}
		\cos x &= \frac {1-t^2}{1+t^2} \\
		\sin x &= \frac{2t}{1+t^2} \\
		\tan x &= \frac{2t}{1-t^2}
	\end{cases}$$
	
	Avec \quad $t=\tanh \frac{x}{2}$ \quad on a \quad
	$$
	\begin{cases}
		\ch x &= \frac {1+t^2}{1-t^2} \\
		\sh x &= \frac{2t}{1-t^2} \\
		\tanh x &= \frac{2t}{1+t^2}
	\end{cases}$$
\end{multicols}

% \vspace{2cm}
\begin{multicols}{2}
	
	
	\begin{align*}
		\cos'x&= -\sin x\\
		\sin'x&=\cos x\\
		\tan' x &= 1+\tan^2x=\frac{1}{\cos^2x}\\
	\end{align*}%\vspace{0.1cm}

\textbf{D\'eriv\'ees}: la multiplication par $\ii$ n'est plus valable
	\begin{align*}
		\ch'x&= \sh x\\
		\sh'x&=\ch x\\
		\tanh' x &= 1-\tanh^2x=\frac{1}{\ch^2x}\\
	\end{align*}
\end{multicols}


\begin{multicols}{2}

	\begin{align*}
		\text{arccos}'x&=\frac{-1}{\sqrt{1-x^2}} \quad (|x|<1)\\
		\text{arcsin}'x&=\frac{1}{\sqrt{1-x^2}} \quad (|x|<1)\\
		\text{arctan}'x&=\frac{1}{1+x^2}
	\end{align*}%\vspace{0.1cm}

	\begin{align*}
		\text{Argch}'x&=\frac{1}{\sqrt{x^2-1}} \quad (x>1)\\
		\text{Argsh}'x&=\frac{1}{\sqrt{x^2+1}} \\
		\text{Argth}'x&=\frac{1}{1-x^2} \quad (|x|<1)
	\end{align*}
	
\end{multicols}



\end{document}	